Unify split and lower operations into update

src/lang/MemoryFacts.v
@@ -16,100 +16,55 @@ Require Import Memory.
 
 Set Implicit Arguments.
 
+(* TODO *)
+Inductive sim_memory (mem_src mem_tgt:Memory.t): Prop :=
+.
 
-Lemma add_lower_add
-      mem1 loc from to val released released' mem2
-      (ADD: Memory.add mem1 loc from to val released mem2)
-      (REL_LE: Capability.le released' released)
-      (REL_WF: Capability.wf released'):
-  exists mem2', Memory.add mem1 loc from to val released' mem2'.
+Lemma add_update_add
+      mem0 loc from1 from2 to val released1 released2 mem1 mem2
+      (ADD1: Memory.add mem0 loc from1 to val released1 mem1)
+      (UPDATE2: Memory.update mem1 loc from1 from2 to val released1 released2 mem2):
+  Memory.add mem0 loc from2 to val released2 mem2.
 Proof.
-  apply Memory.add_exists; auto.
-  - inv ADD. inv ADD0. eauto.
-  - inv ADD. inv ADD0. auto.
-Qed.
+Admitted.
 
-Lemma split_lower_split
-      mem1 loc from to1 to2 val released released' mem2
-      (SPLIT: Memory.split mem1 loc from to1 to2 val released mem2)
-      (REL_LE: Capability.le released' released)
-      (REL_WF: Capability.wf released'):
-  exists mem2', Memory.split mem1 loc from to1 to2 val released' mem2'.
+Lemma update_update_update
+      mem0 loc from0 from1 from2 to val released0 released1 released2 mem1 mem2
+      (UPDATE1: Memory.update mem0 loc from0 from1 to val released0 released1 mem1)
+      (UPDATE2: Memory.update mem1 loc from1 from2 to val released1 released2 mem2):
+  Memory.update mem0 loc from0 from2 to val released0 released2 mem2.
 Proof.
-  exploit Memory.split_get0; eauto. i. des.
-  eapply Memory.split_exists; eauto.
-  - inv SPLIT. inv SPLIT0. auto.
-  - inv SPLIT. inv SPLIT0. auto.
-Qed.
+Admitted.
 
-Lemma lower_lower_lower
-      mem1 loc from to val released0 released released' mem2
-      (LOWER: Memory.lower mem1 loc from to val released0 released mem2)
-      (REL_LE: Capability.le released' released)
-      (REL_WF: Capability.wf released'):
-  exists mem2', Memory.lower mem1 loc from to val released0 released' mem2'.
+Lemma promise_promise_promise
+      loc from1 from2 to val released1 released2 promises0 promises1 promises2 mem0 mem1 mem2 kind
+      (PROMISE1: Memory.promise promises0 mem0 loc from1 to val released1 promises1 mem1 kind)
+      (PROMISE2: Memory.promise promises1 mem1 loc from2 to val released2 promises2 mem2 (Memory.promise_kind_update from1 released1)):
+  Memory.promise promises0 mem0 loc from2 to val released2 promises2 mem2 kind.
 Proof.
-  inv LOWER.
-  exploit add_lower_add; eauto. i. des.
-  esplits. econs; eauto.
-  etrans; eauto.
-Qed.
-
-Lemma promise_lower_promise
-      promises1 mem1 loc from to val released released' promises2 mem2 kind
-      (PROMISE: Memory.promise promises1 mem1 loc from to val released promises2 mem2 kind)
-      (REL_LE: Capability.le released' released)
-      (REL_WF: Capability.wf released'):
-  exists promises2' mem2',
-    Memory.promise promises1 mem1 loc from to val released' promises2' mem2' kind.
-Proof.
-  inv PROMISE.
-  - exploit add_lower_add; try apply PROMISES; eauto. i. des.
-    exploit add_lower_add; try apply MEM; eauto. i. des.
-    esplits. econs; eauto.
-    etrans; eauto. apply REL_LE.
-  - exploit split_lower_split; try apply PROMISES; eauto. i. des.
-    exploit split_lower_split; try apply MEM; eauto. i. des.
-    esplits. econs; eauto.
-    etrans; eauto. apply REL_LE.
-  - exploit lower_lower_lower; try apply PROMISES; eauto. i. des.
-    exploit lower_lower_lower; try apply MEM; eauto. i. des.
-    esplits. econs; eauto.
-Qed.
-
-Lemma write_lower_write
-      promises1 mem1 loc from to val released released' promises2 mem2 kind
-      (WRITE: Memory.write promises1 mem1 loc from to val released promises2 mem2 kind)
-      (REL_LE: Capability.le released' released)
-      (REL_WF: Capability.wf released'):
-  exists promises2' mem2',
-    Memory.write promises1 mem1 loc from to val released' promises2' mem2' kind.
-Proof.
-  inv WRITE. exploit promise_lower_promise; eauto. i. des.
-  exploit Memory.promise_get2; eauto. i.
-  exploit Memory.remove_exists; eauto. i. des.
-  esplits. econs; eauto.
+  inv PROMISE2. inv PROMISE1. 
+  - econs; eauto.
+    + eapply add_update_add; eauto.
+    + eapply add_update_add; eauto.
+  - econs; eauto.
+    + eapply update_update_update; eauto.
+    + eapply update_update_update; eauto.
 Qed.
 
 Lemma remove_promise_remove
       promises0 mem0 loc from to val released1 released2 promises2
       (PRMOISES: Memory.le promises0 mem0)
+      (MEM: Memory.closed mem0)
       (REL_LE: Capability.le released2 released1)
       (REL_WF1: Capability.wf released1)
       (REL_WF2: Capability.wf released2)
       (TIME: Time.lt from to)
       (REMOVE: Memory.remove promises0 loc from to val released1 promises2):
   exists promises1' mem1',
-    <<PROMISE: Memory.promise promises0 mem0 loc from to val released2 promises1' mem1' Memory.promise_kind_lower>> /\
+    <<PROMISE: Memory.promise promises0 mem0 loc from to val released2 promises1' mem1' (Memory.promise_kind_update from released1)>> /\
     <<REMOVE: Memory.remove promises1' loc from to val released2 promises2>> /\
-    <<MEM: Memory.sim mem0 mem1'>>.
+    <<MEM: sim_memory mem1' mem0>>.
 Proof.
-  exploit Memory.remove_get0; eauto. i.
-  exploit Memory.promise_exists_same; try apply x0; eauto. i. des.
-  exploit promise_lower_promise; eauto. i. des.
-  esplits; eauto.
-  - admit. (* Memory.remove *)
-  - inv x2. econs 2; eauto. econs 2. eauto.
 Admitted.
 
 Lemma promise_time_lt
@@ -119,8 +74,7 @@ Lemma promise_time_lt
 Proof.
   inv PROMISE.
   - inv MEM. inv ADD. auto.
-  - inv MEM. inv SPLIT. auto.
-  - inv MEM. inv ADD. inv ADD0. auto.
+  - inv MEM. inv UPDATE. auto.
 Qed.
 
 Lemma write_time_lt
